\documentclass[notitlepage]{simple}

\author{Matt McCarthy\\\href{mailto:matthew.mccarthy.12@cnu.edu}{matthew.mccarthy.12@cnu.edu}}
\title{Derivatives of Arctan at 0}
\date{Februrary, 2016}

\begin{document}
\maketitle

\section{Statement of Problem}

Define $f(x):=\arctan x$.
Find $f^{(n)}(0)$.

\section{Background}

For this problem we will need two theorems.
Firstly, we need Taylor's Theorem.
\begin{thm}[Taylor's Theorem on a disk in $\CC$]\label{t-thm}
	Let $f:\CC\rightarrow\CC$ be analytic on a disk of radius $r$ about $z_0$.
	Then there exists a unique power series such that
	\[
		f(z)=\sum_{k=0}^\infty \frac{f^{(k)}(z_0)}{k!}(z-z_0)^k
	\]
	for all $z$ such that $|z-z_0|<r$.
\end{thm}
Furthermore, we need an additional Taylor expansion.
\begin{thm}\label{t-exp}
	Define
	\[
		f(z):=\frac{1}{1-z}.
	\]
	Then,
	\[
		f(z)=\sum_{k=0}^\infty z^k
	\]
	for any $z\in\CC$ with $|z|<1$.
\end{thm}

\section{Solution}

Define $g(x):=f'(x)$.
We know that
\[
	g(x)=f'(x)=\frac{1}{1+x^2} = \frac{1}{1-(-x^2)}.
\]
From here we can invoke \autoref{t-exp} to get
\[
	g(x) = \sum_{n=0}^\infty (-x^2)^n = \sum_{n=0}^\infty (-1)^n (x-0)^{2n}.
\]
Furthermore, we know that this power series representation is unique by \autoref{t-thm}.
Thus,
\[
	g(x)=\sum_{n=0}^\infty \frac{g^{(n)}(0)}{n!}(x-0)^n=\sum_{n=0}^\infty (-1)^n (x-0)^{2n}.
\]
Using \autoref{t-thm}, we notice that $g^{(2n+1)}(0)=0$ since no odd terms appead in the Taylor expansion.
Moreover, by \autoref{t-thm} we get
\[
	\frac{g^{(2n)}(0)}{(2n)!}=(-1)^n.
\]
Therefore, $g^{(2n)}(0)=(-1)^n(2n)!$.
However, by definition of $g=f'$, we have $f^{(2n+2)}(0)=0$ and $f^{(2n+1)}(0)=(-1)^n(2n)!$.
\end{document}
