\documentclass[notitlepage]{simple}

\author{Matt McCarthy}
\title{Cauchy-Schwarz Inequality}
\date{March 2016}

\begin{document}
	\maketitle
	\begin{thm*}
		Prove that
		\[
			\frac{(a+b)^2}{x+y}\leq \frac{a^2}{x}+\frac{b^2}{y}
		\]
		for $a,b,x,y>0$.
		Use that to the prove the Cauchy-Schwarz inequality,
		\[
			\paren{\sum_{i=0}^n a_ib_i}^2 \leq \paren{\sum_{i=0}^n a_i^2}\paren{\sum_{i=0}^n b_i^2}
		\]
		where $\set{a_i}_{i=0}^n,\set{b_i}_{i=0}^n\subset\RR^+$.
	\end{thm*}

	To begin, we need to prove the following lemma.
	\begin{lemma}
		Let $a,b,x,y>0$, then
		\[
			\frac{(a+b)^2}{x+y}\leq \frac{a^2}{x}+\frac{b^2}{y}.
		\]
	\end{lemma}
	\begin{proof}
		Proceed via contradiction.
		Assume that
		\[
			\frac{(a+b)^2}{x+y}>\frac{a^2}{x}+\frac{b^2}{y}.
		\]
		Then,
		\[
			\frac{(a+b)^2}{x+y}-\frac{a^2}{x}-\frac{b^2}{y}>0.
		\]
		Multiplying out the denominators yields
		\[
			xy(a+b)^2-y(x+y)a^2-x(x+y)b^2>0
		\]
		and thus
		\[
			xya^2+2abxy+xyb^2-xya^2-y^2a^2-xyb^2-x^2b^2>0.
		\]
		Therefore
		\[
			-\paren{(ya)^2-2abxy+(xb)^2}>0
		\]
		and
		\[
			(ya-xb)^2=(ya)^2-2abxy+(xb)^2 < 0.
		\]
		However, $(ya-xb)^2\geq 0$ since $ya-xb\in\RR$.
		This is a contradiction, and thus
		\[
			\frac{(a+b)^2}{x+y}\leq \frac{a^2}{x}+\frac{b^2}{y}.
		\]
	\end{proof}

	We now generalize the previous lemma.
	\begin{lemma}
		Let $a_i,x_i>0$ for all $i$ such that $0\leq i\leq n$.
		Then,
		\[
			\frac{\paren{\sum_{i=0}^na_i}^2}{\sum_{i=0}^n x_i}\leq \sum_{i=0}^n\frac{a_i^2}{x_i}.
		\]
	\end{lemma}
	\begin{proof}
		Proceed via induction.
		Let $H(k)$ represent the hypothesis that the previous statement is true for $n=k$.
		By Lemma 1, $H(1)$ is true.
		Assume $H(n)$ is true.
		We want to show that $H(n+1)$ is true.
		By $H(1)$, we know that
		\[
			\frac{\paren{\sum_{i=0}^{n+1}a_i}^2}{\sum_{i=0}^{n+1} x_i}
			\leq \frac{\paren{\sum_{i=0}^na_i}^2}{\sum_{i=0}^n x_i}+\frac{a_{n+1}^2}{x_{n+1}}.
		\]
		By $H(n)$
		\[
			\frac{\paren{\sum_{i=0}^{n+1}a_i}^2}{\sum_{i=0}^{n+1} x_i}
			\leq \frac{\paren{\sum_{i=0}^na_i}^2}{\sum_{i=0}^n x_i}+\frac{a_{n+1}^2}{x_{n+1}}=
			\leq \sum_{i=0}^n\frac{a_i^2}{x_i}+\frac{a_{n+1}^2}{x_{n+1}}
			=\sum_{i=0}^{n+1}\frac{a_i^2}{x_i}.
		\]
		Thus $H(n+1)$ is true and by induction $H(k)$ is true for all $k$.
	\end{proof}
	This leads us to the Cauchy-Schwarz inequality.
	\begin{thm}
		Let $\set{a_i}_{i=0}^n,\set{b_i}_{i=0}^n\subset\RR^+$, then
		\[
			\paren{\sum_{i=0}^n a_ib_i}^2 \leq \paren{\sum_{i=0}^n a_i^2}\paren{\sum_{i=0}^n b_i^2}.
		\]
	\end{thm}
	\begin{proof}
		Consider the right hand side.
		\[
			\paren{\sum_{i=0}^n a_i^2}\paren{\sum_{j=0}^n b_j^2}=\sum_{k=0}^{2n}\sum_{i+j=k}a_i^2b_j^2
		\]
		Since these are all nonnegative, we can drop the odd terms
		\[
			\paren{\sum_{i=0}^n a_i^2}\paren{\sum_{j=0}^n b_j^2}
			=\sum_{k=0}^{2n}\sum_{i+j=k}a_i^2b_j^2
			\geq \sum_{k=0}^{n}\sum_{i+j=2k}a_i^2b_j^2.
		\]
		Furthermore, $k+k=2k$ and thus
		\[
			\paren{\sum_{i=0}^n a_i^2}\paren{\sum_{j=0}^n b_j^2}
			\geq \sum_{k=0}^{n}\sum_{i+j=2k}a_i^2b_j^2
			\geq \sum_{k=0}^{n}a_k^2b_k^2.
		\]
		Consider
		\[
			\paren{\sum_{i=0}^n a_ib_i}^2.
		\]
		Then,
		\[
			\paren{\sum_{i=0}^n a_ib_i}^2
			= \frac{\paren{\sum_{i=0}^n a_ib_i}^2}{\sum_{i=0}^n\frac{1}{n+1}}.
		\]
		If we invoke Lemma 2,
		\[
			\paren{\sum_{i=0}^n a_ib_i}^2
			= \frac{\paren{\sum_{i=0}^n a_ib_i}^2}{\sum_{i=0}^n\frac{1}{n+1}}
			\leq \sum_{i=0}^n a_i^2b_i^2(n+1)
			\leq \sum_{i=0}^n a_i^2b_i^2
			\leq\paren{\sum_{i=0}^n a_i^2}\paren{\sum_{i=0}^n b_i^2}.
		\]
	\end{proof}
\end{document}
